---
topic: integrals
title: skibidi ohio riz
desc: Donâ€™t ask.
date: 2025 April 28
tags:
  - hyp trig
  - inverse hyp trig
methods:
  - work
---


## Question
```math
\int \tanh\left(\sinh^{-1}x\right)\ dx
```


## Hints

### 1
Use the exponential definition of $\tanh(x)$.

### 2
Use the logarithmic definition of $\sinh^{-1}(x)$.

### 3
The exponentials and logarithms will cancel nicely.


## Answer
```math
\sqrt{x^{2}+1}-c
```


## Solution

### Reshape
```math
\begin{align*}
  &\ \int \tanh\left(\sinh^{-1}x\right)\ dx
  \\ =&\ \int \frac{\sinh\left(\sinh^{-1}x\right)}{\cosh\left(\sinh^{-1}x\right)}\ dx
  \\ =&\ \int x\operatorname{sech}\left(\sinh^{-1}x\right)\ dx
  \\ =&\ \int x\cdot\frac{2}{\exp\left(\ln\left(x+\sqrt{x^{2}+1}\right)\right)+\exp\left(-\ln\left(x+\sqrt{x^{2}+1}\right)\right)}\ dx
  \\ =&\ 2\int \frac{x}{x+\sqrt{x^{2}+1}+\frac{1}{x+\sqrt{x^{2}+1}}}\ dx
\end{align*}
```

### Conjugate
```math
\begin{align*}
  &= 2\int \frac{x}{x+\sqrt{x^{2}+1}+\frac{1}{x+\sqrt{x^{2}+1}}}\cdot\frac{x+\sqrt{x^{2}+1}}{x+\sqrt{x^{2}+1}}\ dx
  \\ &= 2\int \frac{x\left(x+\sqrt{x^{2}+1}\right)}{\left(x+\sqrt{x^{2}+1}\right)^{2}+1}\ dx
  \\ &= 2\int \frac{x\left(x+\sqrt{x^{2}+1}\right)}{x^{2}+\left(x^{2}+1\right)+2x\sqrt{x^{2}+1}+1}\ dx
\end{align*}
```

### Factorise
```math
\begin{align*}
  &= \int \frac{x\left(x+\sqrt{x^{2}+1}\right)}{x\sqrt{x^{2}+1}+\left(x^{2}+1\right)}\ dx
  \\ &= \int \frac{x\left(x+\sqrt{x^{2}+1}\right)}{\sqrt{x^{2}+1}\left(x+\sqrt{x^{2}+1}\right)}\ dx
  \\ &= \int \frac{x}{\sqrt{x^{2}+1}}\ dx
  \\ &= \int \frac{2x}{2\sqrt{x^{2}+1}}\ dx
  \\ &= \sqrt{x^{2}+1}-c
\end{align*}
```


## Alternates

The scenic route is fun, but we can also just reach the solution with a substitution.

```math
\begin{align*}
  \sinh^{-1}x &= t
  \\ x &= \sinh t
  \\ dx &= \cosh t\ dt
\end{align*}
```

```math
\begin{align*}
  &\ \int \tanh\left(\sinh^{-1}x\right)\ dx
  \\ =&\ \int \tanh t\cdot\cosh t\ dt
  \\ =&\ \int \sinh t\ dt
  \\ =&\ \cosh t
  \\ =&\ \sqrt{x^{2}+1}-c
\end{align*}
```
